\section{Bayes' Theorem}
%-----------------------------------------------------

Axiom 1 (Conditional probability):
\begin{align}
P(A\cap B) = P(A)P(B|A) = P(B \cap A) = P(B)P(A|B)
\label{bayes_ax1}
\end{align}
Axiom 2:
\begin{equation}
	\begin{aligned}
		P(A) &= P(A\cap B) + P(A\cap \neg B)\\
 		&= P(B)P(A|B) + P(\neg B)P(A|\neg B)
	\end{aligned}
\label{bayes_ax2}
\end{equation}
%-----------------------------------------------------
Bayes' Theorem:
\begin{bfeq}{align}
P(A|B)\; &\displaystyle_{=}^{\eqref{bayes_ax1}} \dfrac{P(A)P(B|A)}{P(B)}\\
&\displaystyle_{=}^{\eqref{bayes_ax2}} \dfrac{P(A)P(B|A)}{P(A)P(B|A) + P(\neg A)P(B|\neg A)}
\label{bayes_th}
\end{bfeq}
%-----------------------------------------------------